oPCF/Operation.lean
@@ -1,67 +1,18 @@
 import «oPCF».Syntax
 
-def Ren Γ Δ := {τ : Ty} → Var Γ τ → Var Δ τ
-def Reb Γ Δ := {τ : Ty} → Tm Γ τ → Tm Δ τ
-
-def extend_ren (r : Ren Γ Δ) {τ  : Ty} : Ren (Γ ∷ τ) (Δ ∷ τ) :=
-  fun v => match v with
-  | .z => .z
-  | .s x => .s (r x)
-
-def rename (r : Ren Γ Δ) : Reb Γ Δ :=
-  fun dv => match dv with
-  | .var x => .var (r x)
-  | .true => .true
-  | .false => .false
-  | .zero => .zero
-  | .succ e => (rename r e).succ
-  | .pred e => (rename r e).pred
-  | .zero? e => (rename r e).zero?
-  | .cond s et ef => (rename r s).cond (rename r et) (rename r ef)
-  | .fn e => (rename (extend_ren r) e).fn
-  | .app f a => (rename r f).app (rename r a)
-  | .fix f => (rename r f).fix
-
-def Subst Γ Δ := {τ : Ty} → Var Γ τ → Tm Δ τ
-
-def extend_subst (σ : Subst Γ Δ) {τ : Ty} : Subst (Γ ∷ τ) (Δ ∷ τ) :=
-  fun dv => match dv with
-  | .z => .var .z
-  | .s x => rename .s (σ x)
-
-def subst (σ : Subst Γ Δ) : Reb Γ Δ :=
-  fun {τ} e => match e with
-  | .var x => σ x
-  | .true => .true
-  | .false => .false
-  | .zero => .zero
-  | .succ e => (subst σ e).succ
-  | .pred e => (subst σ e).pred
-  | .zero? e => (subst σ e).zero?
-  | .cond s et ef => (subst σ s).cond (subst σ et) (subst σ ef)
-  | .fn e => (subst (extend_subst σ) e).fn
-  | .app f a => (subst σ f).app (subst σ a)
-  | .fix f => (subst σ f).fix
-
-def sb1 (a : Tm Γ υ) : Subst (Γ ∷ υ) Γ := fun v => match v with
-  | .z => a
-  | .s x => .var x
-
-def subst_1 (e : Tm (Γ ∷ τ) υ) (a : Tm Γ τ) : Tm Γ υ
-  :=subst (sb1 a) e
-
-inductive Eval : Tm .nil τ → Tm .nil τ → Type
+inductive Eval : (.nil ⊢ τ) → (.nil ⊢ τ) → Type
   | true : Eval .true .true
   | false : Eval .false .false
   | zero : Eval .zero .zero
   | succ : Eval t v → Eval (t.succ) (v.succ)
   | fn : Eval (.fn e) (e.fn)
-  | pred : Eval t (.succ v) → Eval (.pred t) (v)
+  | pred : Tm.is_value v → Eval t (v.succ) → Eval (.pred t) (v)
   | zero?_zero : Eval t (.zero) → Eval (t.zero?) .true
-  | zero?_succ : Eval t (.succ v) → Eval (t.zero?) .false
+  | zero?_succ : Tm.is_value v → Eval t (v.succ) → Eval (t.zero?) .false
   | cond_true {t ct cf vt} : Eval t (.true) → Eval ct vt → Eval (t.cond ct cf) vt
   | cond_false {t ct cf vf} : Eval t (.false) → Eval cf vf → Eval (t.cond ct cf) vf
-  | app : Eval f (e.fn) → Eval (subst_1 e u) v → Eval (f.app u) v
+  | app {e : Tm ..} : Eval f (e.fn) → Eval (e.sub (sb1 u)) v → Eval (f.app u) v
+  | fix {f : Tm ..} : Eval (f.app f.fix) v → Eval (f.fix) v
 
 infixl:75 " ⇓ " => Eval
 
@@ -85,15 +36,15 @@ theorem determinism : t ⇓ v₀ → t ⇓ v₁ → v₀ = v₁ := by
   | fn =>
     cases h₁
     rfl
-  | pred _ Φ =>
+  | pred _ _ Φ =>
     cases h₁
     case _ _ x =>
     injection Φ x
   | zero?_zero _ Φ =>
     cases h₁ with
     | zero?_zero => rfl
-    | zero?_succ x => injection Φ x
-  | zero?_succ _ Φ =>
+    | zero?_succ _ x => injection Φ x
+  | zero?_succ _ _ Φ =>
     cases h₁ with
     | zero?_zero x => injection Φ x
     | zero?_succ x => rfl
@@ -111,3 +62,7 @@ theorem determinism : t ⇓ v₀ → t ⇓ v₁ → v₀ = v₁ := by
     injection Φ₀ x₀ with _ _ _ p
     rw [←p] at x₁
     exact Φ₁ x₁
+  | fix _ Φ =>
+    cases h₁
+    case _ x₀ =>
+    exact Φ x₀
