oPCF/Syntax.lean
@@ -28,4 +28,71 @@ inductive Tm : Cx → Ty → Type
   | app : Tm Γ (τ ⇒ υ) → Tm Γ τ → Tm Γ υ
   | fix : Tm Γ (τ ⇒ τ) → Tm Γ τ
 
-notation:10 Γ "⊢" τ => Tm Γ τ
+notation:10 Γ " ⊢ " τ => Tm Γ τ
+
+def Tm.from_bool : Bool → (Γ ⊢ .bool)
+  | .true => .true
+  | .false => .false
+
+def Tm.from_nat : Nat → (Γ ⊢ .nat)
+  | .zero => .zero
+  | .succ n => .succ (Tm.from_nat n)
+
+inductive Tm.is_value : (Γ ⊢ τ) → Type
+  | true : true.is_value
+  | false : false.is_value
+  | zero : zero.is_value
+  | succ {v : Tm ..} : v.is_value → v.succ.is_value
+  | fn {e : Tm ..} : e.fn.is_value
+
+
+def Ren Γ Δ := ∀ {τ}, Var Γ τ → Var Δ τ
+def Reb Γ Δ := {τ : Ty} → Tm Γ τ → Tm Δ τ
+
+def extend_ren (r : Ren Γ Δ) {τ  : Ty} : Ren (Γ ∷ τ) (Δ ∷ τ) :=
+  fun v => match v with
+  | .z => .z
+  | .s x => .s (r x)
+
+def rename (r : Ren Γ Δ) : Reb Γ Δ :=
+  fun dv => match dv with
+  | .var x => .var (r x)
+  | .true => .true
+  | .false => .false
+  | .zero => .zero
+  | .succ e => (rename r e).succ
+  | .pred e => (rename r e).pred
+  | .zero? e => (rename r e).zero?
+  | .cond s et ef => (rename r s).cond (rename r et) (rename r ef)
+  | .fn e => (rename (extend_ren r) e).fn
+  | .app f a => (rename r f).app (rename r a)
+  | .fix f => (rename r f).fix
+
+def Tm.ren (t : Γ ⊢ τ) (r : Ren Γ Δ) : Δ ⊢ τ := rename r t
+
+def Subst Γ Δ := ∀ τ, Var Γ τ → Tm Δ τ
+
+def extend_subst (σ : Subst Γ Δ) {τ : Ty} : Subst (Γ ∷ τ) (Δ ∷ τ) :=
+  fun τ x => match x with
+  | .z => .var .z
+  | .s x => (σ τ x).ren .s
+
+def subst (σ : Subst Γ Δ) : Reb Γ Δ :=
+  fun {τ} e => match e with
+  | .var x => σ τ x
+  | .true => .true
+  | .false => .false
+  | .zero => .zero
+  | .succ e => (subst σ e).succ
+  | .pred e => (subst σ e).pred
+  | .zero? e => (subst σ e).zero?
+  | .cond s et ef => (subst σ s).cond (subst σ et) (subst σ ef)
+  | .fn e => (subst (extend_subst σ) e).fn
+  | .app f a => (subst σ f).app (subst σ a)
+  | .fix f => (subst σ f).fix
+
+def Tm.sub (t : Γ ⊢ τ) (σ : Subst Γ Δ) : Δ ⊢ τ := subst σ t
+
+def sb1 (a : Tm Γ υ) : Subst (Γ ∷ υ) Γ := fun τ v => match v with
+  | .z => a
+  | .s x => .var x
