lakefile.lean
@@ -6,8 +6,5 @@ package «oPCF» where
     ⟨`pp.unicode.fun, true⟩ -- pretty-prints `fun a ↦ b`
   ]
 
-require mathlib from git
-  "https://github.com/leanprover-community/mathlib4.git"
-
 @[default_target]
 lean_lib «oPCF» where
