oPCF/Utility.lean
@@ -1,0 +1,7 @@
+def Nat.zero? : Nat → Bool
+| .zero => true
+| _ => false
+
+theorem Nat.pred_succ_id : Nat.pred ∘ Nat.succ = id := by
+  apply funext
+  exact Nat.pred_succ
